More precise error messages.

deps/coq-poulet4/lib/Unpack.v
@@ -22,91 +22,112 @@ Section Unpack.
   Notation P4String := (P4String.t tags_t).
   Notation P4Int := (P4Int.t tags_t).
   Notation P4Parameter := (@Typed.P4Parameter tags_t).
+
   Definition unpack_bool (wrapped: env_monad Value) : env_monad bool :=
     let* unwrapped := wrapped in
     match unwrapped with
     | ValBase (ValBaseBool b) => mret b
-    | _ => state_fail Internal
+    | _ => state_fail (TypeError "Cannot unpack value as boolean.")
     end.
 
   (* TODO: unpack_fixed_bit, unpack_var_bit; dependent types make things hard here *)
+
+  Definition unpack_fixed_bits (wrapped: env_monad Value) : env_monad (nat * Z) :=
+    let* unwrapped := wrapped in
+    match unwrapped with
+    | ValBase (ValBaseBit w n) => state_return (w, n)
+    | _ => state_fail (TypeError "Cannot unpack value as fixed-with bits.")
+    end.
+
+  Definition unpack_var_bits (wrapped: env_monad Value) : env_monad (nat * nat * Z) :=
+    let* unwrapped := wrapped in
+    match unwrapped with
+    | ValBase (ValBaseVarbit m w n) => state_return (m, w, n)
+    | _ => state_fail (TypeError "Cannot unpack value as variable-width bits.")
+    end.
+
   Definition unpack_fixed_int (wrapped: env_monad Value) : env_monad (nat * Z) :=
     let* unwrapped := wrapped in
     match unwrapped with
-    | ValBase (ValBaseInt w n) => (state_return (w, n):env_monad (nat*Z))
-    | _ => state_fail Internal
+    | ValBase (ValBaseInt w n) => state_return (w, n)
+    | _ => state_fail (TypeError "Cannot unpack value as fixed-width integer.")
     end.
 
   Definition unpack_inf_int (wrapped: env_monad Value) : env_monad Z :=
     let* unwrapped := wrapped in
     match unwrapped with
     | ValBase (ValBaseInteger n) => mret n
-    | _ => state_fail Internal
+    | _ => state_fail (TypeError "Cannot unpack value as variable-width integer.")
     end.
 
   Definition unpack_string (wrapped: env_monad Value) : env_monad String.t :=
     let* unwrapped := wrapped in
     match unwrapped with
     | ValBase (ValBaseString s) => mret s.(P4String.str)
-    | _ => state_fail Internal
+    | _ => state_fail (TypeError "Cannot unpack value as string")
     end.
 
   Definition unpack_array (wrapped: env_monad Value) : env_monad (list ValueBase) :=
     let* unwrapped := wrapped in
     match unwrapped with
     | ValBase (ValBaseTuple vals) => mret vals
-    | _ => state_fail Internal
+    | _ => state_fail (TypeError "Cannot unpack value as tuple.")
     end.
 
   Definition unpack_error (wrapped: env_monad Value) : env_monad P4String :=
     let* unwrapped := wrapped in
     match unwrapped with
     | ValBase (ValBaseError e) => mret e
-    | _ => state_fail Internal
+    | _ => state_fail (TypeError "Cannot unpack value as error.")
     end.
 
   Definition unpack_record (wrapped: env_monad Value) :=
     let* unwrapped := wrapped in
     match unwrapped with
     | ValBase (ValBaseRecord fs) => mret fs
-    | _ => state_fail Internal
+    | _ => state_fail (TypeError "Cannot unpack value as record.")
     end.
 
   Definition unpack_func (wrapped: env_monad Value) : env_monad (list P4Parameter * ValueFunctionImplementation) :=
     let* unwrapped := wrapped in
     match unwrapped with
     | ValObj (ValObjFun params impl) => mret (params, impl)
-    | _ => state_fail Internal
+    | _ => state_fail (TypeError "Cannot unpack value as function")
     end.
 
   Definition unpack_extern_obj (wrapped: env_monad Value) : env_monad (list (P4String * list P4Parameter)) :=
     let* unwrapped := wrapped in
     match unwrapped with
     | ValCons (ValConsExternObj e) => mret e
-    | _ => state_fail Internal
+    | _ => state_fail (TypeError "Cannot unpack value as extern object.")
     end.
 
-  Set Printing All.
+  Definition unpack_packet (wrapped: env_monad Value) : env_monad (list bool) :=
+    let* unwrapped := wrapped in
+    match unwrapped with
+    | ValObj (ValObjPacket e) => mret e
+    | _ => state_fail (TypeError "Cannot unpack value as packet.")
+    end.
 
   Definition unpack_header (wrapped: env_monad Value) : env_monad (list (P4String * ValueBase) * bool) :=
     let* unwrapped := wrapped in
     match unwrapped with
     | ValBase (ValBaseHeader h v) => mret (h, v)
-    | _ => state_fail Internal
+    | _ => state_fail (TypeError "Cannot unpack value as header.")
     end.
 
   Definition unpack_header_stack (wrapped: env_monad Value) : env_monad (list ValueBase * nat * nat) :=
     let* unwrapped := wrapped in
     match unwrapped with
     | ValBase (ValBaseStack hdrs size next)  => mret (hdrs, size, next)
-    | _ => state_fail Internal
+    | _ => state_fail (TypeError "Cannot unpack value as header stack.")
     end.
 
   Definition unpack_lvalue (wrapped: env_monad Value) : env_monad (ValueLvalue) :=
     let* unwrapped := wrapped in
     match unwrapped with
     | ValLvalue lvalue  => mret lvalue
-    | _ => state_fail Internal
+    | _ => state_fail (TypeError "Cannot unpack value as lvalue.")
     end.
 
 End Unpack.
